added invariant proofs to AA trees

src/HOL/Data_Structures/AA_Set.thy
@@ -1,7 +1,5 @@
 (*
-Author: Tobias Nipkow
-
-Added trivial cases to function `adjust' to obviate invariants.
+Author: Tobias Nipkow and Daniel Stüwe
 *)
 
 section \<open>AA Tree Implementation of Sets\<close>
@@ -17,13 +15,13 @@ type_synonym 'a aa_tree = "('a,nat) tree"
 fun lvl :: "'a aa_tree \<Rightarrow> nat" where
 "lvl Leaf = 0" |
 "lvl (Node lv _ _ _) = lv"
-(*
+
 fun invar :: "'a aa_tree \<Rightarrow> bool" where
 "invar Leaf = True" |
 "invar (Node h l a r) =
  (invar l \<and> invar r \<and>
   h = lvl l + 1 \<and> (h = lvl r + 1 \<or> (\<exists>lr b rr. r = Node h lr b rr \<and> h = lvl rr + 1)))"
-*)
+
 fun skew :: "'a aa_tree \<Rightarrow> 'a aa_tree" where
 "skew (Node lva (Node lvb t1 b t2) a t3) =
   (if lva = lvb then Node lva t1 b (Node lva t2 a t3) else Node lva (Node lvb t1 b t2) a t3)" |
@@ -46,11 +44,6 @@ fun insert :: "'a::cmp \<Rightarrow> 'a aa_tree \<Rightarrow> 'a aa_tree" where
      GT \<Rightarrow> split (skew (Node lv t1 a (insert x t2))) |
      EQ \<Rightarrow> Node lv t1 x t2)"
 
-(* wrong in paper! *)
-fun del_max :: "'a aa_tree \<Rightarrow> 'a aa_tree * 'a" where
-"del_max (Node lv l a Leaf) = (l,a)" |
-"del_max (Node lv l a r) = (let (r',b) = del_max r in (Node lv l a r', b))"
-
 fun sngl :: "'a aa_tree \<Rightarrow> bool" where
 "sngl Leaf = False" |
 "sngl (Node _ _ _ Leaf) = True" |
@@ -65,19 +58,28 @@ definition adjust :: "'a aa_tree \<Rightarrow> 'a aa_tree" where
     if lvl r < lv-1
     then case l of
            Node lva t1 a (Node lvb t2 b t3)
-             \<Rightarrow> Node (lvb+1) (Node lva t1 a t2) b (Node (lv-1) t3 x r) |
-           _ \<Rightarrow> t (* unreachable *)
+             \<Rightarrow> Node (lvb+1) (Node lva t1 a t2) b (Node (lv-1) t3 x r) 
     else
     if lvl r < lv then split (Node (lv-1) l x r)
     else
       case r of
-        Leaf \<Rightarrow> Leaf (* unreachable *) |
         Node lvb t1 b t4 \<Rightarrow>
           (case t1 of
              Node lva t2 a t3
                \<Rightarrow> Node (lva+1) (Node (lv-1) l x t2) a
-                    (split (Node (if sngl t1 then lva-1 else lva) t3 b t4))
-           | _ \<Rightarrow> t (* unreachable *))))"
+                    (split (Node (if sngl t1 then lva else lva+1) t3 b t4)))))"
+
+text{* In the paper, the last case of @{const adjust} is expressed with the help of an
+incorrect auxiliary function \texttt{nlvl}.
+
+Function @{text del_max} below is called \texttt{dellrg} in the paper.
+The latter is incorrect for two reasons: \texttt{dellrg} is meant to delete the largest
+element but recurses on the left instead of the right subtree; the invariant
+is not restored.*}
+
+fun del_max :: "'a aa_tree \<Rightarrow> 'a aa_tree * 'a" where
+"del_max (Node lv l a Leaf) = (l,a)" |
+"del_max (Node lv l a r) = (let (r',b) = del_max r in (adjust(Node lv l a r'), b))"
 
 fun delete :: "'a::cmp \<Rightarrow> 'a aa_tree \<Rightarrow> 'a aa_tree" where
 "delete _ Leaf = Leaf" |
@@ -88,8 +90,367 @@ fun delete :: "'a::cmp \<Rightarrow> 'a aa_tree \<Rightarrow> 'a aa_tree" where
      EQ \<Rightarrow> (if l = Leaf then r
             else let (l',b) = del_max l in adjust (Node lv l' b r)))"
 
+fun pre_adjust where
+"pre_adjust (Node lv l a r) = (invar l \<and> invar r \<and>
+    ((lv = lvl l + 1 \<and> (lv = lvl r + 1 \<or> lv = lvl r + 2 \<or> lv = lvl r \<and> sngl r)) \<or>
+     (lv = lvl l + 2 \<and> (lv = lvl r + 1 \<or> lv = lvl r \<and> sngl r))))"
+
+declare pre_adjust.simps [simp del]
+
+subsection "Auxiliary Proofs"
+
+lemma split_case: "split t = (case t of
+  Node lvx a x (Node lvy b y (Node lvz c z d)) \<Rightarrow>
+   (if lvx = lvy \<and> lvy = lvz
+    then Node (lvx+1) (Node lvx a x b) y (Node lvx c z d)
+    else t)
+  | t \<Rightarrow> t)"
+by(auto split: tree.split)
+
+lemma skew_case: "skew t = (case t of
+  Node lvx (Node lvy a y b) x c \<Rightarrow>
+  (if lvx = lvy then Node lvx a y (Node lvx b x c) else t)
+ | t \<Rightarrow> t)"
+by(auto split: tree.split)
+
+lemma lvl_0_iff: "invar t \<Longrightarrow> lvl t = 0 \<longleftrightarrow> t = Leaf"
+by(cases t) auto
+
+lemma lvl_Suc_iff: "lvl t = Suc n \<longleftrightarrow> (\<exists> l a r. t = Node (Suc n) l a r)"
+by(cases t) auto
+
+lemma lvl_skew: "lvl (skew t) = lvl t"
+by(induction t rule: skew.induct) auto
+
+lemma lvl_split: "lvl (split t) = lvl t \<or> lvl (split t) = lvl t + 1 \<and> sngl (split t)"
+by(induction t rule: split.induct) auto
+
+lemma invar_2Nodes:"invar (Node lv l x (Node rlv rl rx rr)) =
+     (invar l \<and> invar \<langle>rlv, rl, rx, rr\<rangle> \<and> lv = Suc (lvl l) \<and>
+     (lv = Suc rlv \<or> rlv = lv \<and> lv = Suc (lvl rr)))"
+by simp
+
+lemma invar_NodeLeaf[simp]:
+  "invar (Node lv l x Leaf) = (invar l \<and> lv = Suc (lvl l) \<and> lv = Suc 0)"
+by simp
+
+lemma sngl_if_invar: "invar (Node n l a r) \<Longrightarrow> n = lvl r \<Longrightarrow> sngl r"
+by(cases r rule: sngl.cases) clarsimp+
+
+
+subsection "Invariance"
+
+subsubsection "Proofs for insert"
+
+lemma lvl_insert_aux:
+  "lvl (insert x t) = lvl t \<or> lvl (insert x t) = lvl t + 1 \<and> sngl (insert x t)"
+apply(induction t)
+apply (auto simp: lvl_skew)
+apply (metis Suc_eq_plus1 lvl.simps(2) lvl_split lvl_skew)+
+done
+
+lemma lvl_insert: obtains
+  (Same) "lvl (insert x t) = lvl t" |
+  (Incr) "lvl (insert x t) = lvl t + 1" "sngl (insert x t)"
+using lvl_insert_aux by blast
+
+lemma lvl_insert_sngl: "invar t \<Longrightarrow> sngl t \<Longrightarrow> lvl(insert x t) = lvl t"
+proof (induction t rule: "insert.induct" )
+  case (2 x lv t1 a t2)
+  consider (LT) "x < a" | (GT) "x > a" | (EQ) "x = a" 
+    using less_linear by blast 
+  thus ?case proof cases
+    case LT
+    thus ?thesis using 2 by (auto simp add: skew_case split_case split: tree.splits)
+  next
+    case GT
+    thus ?thesis using 2 proof (cases t1)
+      case Node
+      thus ?thesis using 2 GT  
+        apply (auto simp add: skew_case split_case split: tree.splits)
+        by (metis less_not_refl2 lvl.simps(2) lvl_insert_aux n_not_Suc_n sngl.simps(3))+ 
+    qed (auto simp add: lvl_0_iff)
+  qed simp
+qed simp
+
+lemma skew_invar: "invar t \<Longrightarrow> skew t = t"
+by(induction t rule: skew.induct) auto
+
+lemma split_invar: "invar t \<Longrightarrow> split t = t"
+by(induction t rule: split.induct) clarsimp+
+
+lemma invar_NodeL:
+  "\<lbrakk> invar(Node n l x r); invar l'; lvl l' = lvl l \<rbrakk> \<Longrightarrow> invar(Node n l' x r)"
+by(auto)
+
+lemma invar_NodeR:
+  "\<lbrakk> invar(Node n l x r); n = lvl r + 1; invar r'; lvl r' = lvl r \<rbrakk> \<Longrightarrow> invar(Node n l x r')"
+by(auto)
+
+lemma invar_NodeR2:
+  "\<lbrakk> invar(Node n l x r); sngl r'; n = lvl r + 1; invar r'; lvl r' = n \<rbrakk> \<Longrightarrow> invar(Node n l x r')"
+by(cases r' rule: sngl.cases) clarsimp+
+
+
+lemma lvl_insert_incr_iff: "(lvl(insert a t) = lvl t + 1) \<longleftrightarrow>
+  (EX l x r. insert a t = Node (lvl t + 1) l x r \<and> lvl l = lvl r)"
+apply(cases t)
+apply(auto simp add: skew_case split_case split: if_splits)
+apply(auto split: tree.splits if_splits)
+done
+
+lemma invar_insert: "invar t \<Longrightarrow> invar(insert a t)"
+proof(induction t)
+  case (Node n l x r)
+  hence il: "invar l" and ir: "invar r" by auto
+  note N = Node
+  let ?t = "Node n l x r"
+  have "a < x \<or> a = x \<or> x < a" by auto
+  moreover
+  { assume "a < x"
+    note iil = Node.IH(1)[OF il]
+    have ?case
+    proof (cases rule: lvl_insert[of a l])
+      case (Same) thus ?thesis
+        using \<open>a<x\<close> invar_NodeL[OF Node.prems iil Same]
+        by (simp add: skew_invar split_invar del: invar.simps)
+    next
+      case (Incr)
+      then obtain t1 w t2 where ial[simp]: "insert a l = Node n t1 w t2"
+        using Node.prems by (auto simp: lvl_Suc_iff)
+      have l12: "lvl t1 = lvl t2"
+        by (metis Incr(1) ial lvl_insert_incr_iff tree.inject)
+      have "insert a ?t = split(skew(Node n (insert a l) x r))"
+        by(simp add: \<open>a<x\<close>)
+      also have "skew(Node n (insert a l) x r) = Node n t1 w (Node n t2 x r)"
+        by(simp)
+      also have "invar(split \<dots>)"
+      proof (cases r)
+        case Leaf
+        hence "l = Leaf" using Node.prems by(auto simp: lvl_0_iff)
+        thus ?thesis using Leaf ial by simp
+      next
+        case [simp]: (Node m t3 y t4)
+        show ?thesis (*using N(3) iil l12 by(auto)*)
+        proof cases
+          assume "m = n" thus ?thesis using N(3) iil by(auto)
+        next
+          assume "m \<noteq> n" thus ?thesis using N(3) iil l12 by(auto)
+        qed
+      qed
+      finally show ?thesis .
+    qed
+  }
+  moreover
+  { assume "x < a"
+    note iir = Node.IH(2)[OF ir]
+    from \<open>invar ?t\<close> have "n = lvl r \<or> n = lvl r + 1" by auto
+    hence ?case
+    proof
+      assume 0: "n = lvl r"
+      have "insert a ?t = split(skew(Node n l x (insert a r)))"
+        using \<open>a>x\<close> by(auto)
+      also have "skew(Node n l x (insert a r)) = Node n l x (insert a r)"
+        using Node.prems by(simp add: skew_case split: tree.split)
+      also have "invar(split \<dots>)"
+      proof -
+        from lvl_insert_sngl[OF ir sngl_if_invar[OF \<open>invar ?t\<close> 0], of a]
+        obtain t1 y t2 where iar: "insert a r = Node n t1 y t2"
+          using Node.prems 0 by (auto simp: lvl_Suc_iff)
+        from Node.prems iar 0 iir
+        show ?thesis by (auto simp: split_case split: tree.splits)
+      qed
+      finally show ?thesis .
+    next
+      assume 1: "n = lvl r + 1"
+      hence "sngl ?t" by(cases r) auto
+      show ?thesis
+      proof (cases rule: lvl_insert[of a r])
+        case (Same)
+        show ?thesis using \<open>x<a\<close> il ir invar_NodeR[OF Node.prems 1 iir Same]
+          by (auto simp add: skew_invar split_invar)
+      next
+        case (Incr)
+        thus ?thesis using invar_NodeR2[OF `invar ?t` Incr(2) 1 iir] 1 \<open>x < a\<close>
+          by (auto simp add: skew_invar split_invar split: if_splits)
+      qed
+    qed
+  }
+  moreover { assume "a = x" hence ?case using Node.prems by auto }
+  ultimately show ?case by blast
+qed simp
+
+
+subsubsection "Proofs for delete"
+
+lemma invarL: "ASSUMPTION(invar \<langle>lv, l, a, r\<rangle>) \<Longrightarrow> invar l"
+by(simp add: ASSUMPTION_def)
+
+lemma invarR: "ASSUMPTION(invar \<langle>lv, l, a, r\<rangle>) \<Longrightarrow> invar r"
+by(simp add: ASSUMPTION_def)
+
+lemma sngl_NodeI:
+  "sngl (Node lv l a r) \<Longrightarrow> sngl (Node lv l' a' r)"
+by(cases r) (simp_all)
+
+
+declare invarL[simp] invarR[simp]
+
+lemma pre_cases:
+assumes "pre_adjust (Node lv l x r)"
+obtains
+ (tSngl) "invar l \<and> invar r \<and>
+    lv = Suc (lvl r) \<and> lvl l = lvl r" |
+ (tDouble) "invar l \<and> invar r \<and>
+    lv = lvl r \<and> Suc (lvl l) = lvl r \<and> sngl r " |
+ (rDown) "invar l \<and> invar r \<and>
+    lv = Suc (Suc (lvl r)) \<and>  lv = Suc (lvl l)" |
+ (lDown_tSngl) "invar l \<and> invar r \<and>
+    lv = Suc (lvl r) \<and> lv = Suc (Suc (lvl l))" |
+ (lDown_tDouble) "invar l \<and> invar r \<and>
+    lv = lvl r \<and> lv = Suc (Suc (lvl l)) \<and> sngl r"
+using assms unfolding pre_adjust.simps
+by auto
+
+declare invar.simps(2)[simp del] invar_2Nodes[simp add]
+
+lemma invar_adjust:
+  assumes pre: "pre_adjust (Node lv l a r)"
+  shows  "invar(adjust (Node lv l a r))"
+using pre proof (cases rule: pre_cases)
+  case (tDouble) thus ?thesis unfolding adjust_def by (cases r) (auto simp: invar.simps(2)) 
+next 
+  case (rDown)
+  from rDown obtain llv ll la lr where l: "l = Node llv ll la lr" by (cases l) auto
+  from rDown show ?thesis unfolding adjust_def by (auto simp: l invar.simps(2) split: tree.splits)
+next
+  case (lDown_tDouble)
+  from lDown_tDouble obtain rlv rr ra rl where r: "r = Node rlv rl ra rr" by (cases r) auto
+  from lDown_tDouble and r obtain rrlv rrr rra rrl where
+    rr :"rr = Node rrlv rrr rra rrl" by (cases rr) auto
+  from  lDown_tDouble show ?thesis unfolding adjust_def r rr
+    apply (cases rl) apply (auto simp add: invar.simps(2))
+    using lDown_tDouble by (auto simp: split_case lvl_0_iff  elim:lvl.elims split: tree.split)
+qed (auto simp: split_case invar.simps(2) adjust_def split: tree.splits)
+
+lemma lvl_adjust:
+  assumes "pre_adjust (Node lv l a r)"
+  shows "lv = lvl (adjust(Node lv l a r)) \<or> lv = lvl (adjust(Node lv l a r)) + 1"
+using assms(1) proof(cases rule: pre_cases)
+  case lDown_tSngl thus ?thesis
+    using lvl_split[of "\<langle>lvl r, l, a, r\<rangle>"] by (auto simp: adjust_def)
+next
+  case lDown_tDouble thus ?thesis
+    by (auto simp: adjust_def invar.simps(2) split: tree.split)
+qed (auto simp: adjust_def split: tree.splits)
+
+lemma sngl_adjust: assumes "pre_adjust (Node lv l a r)"
+  "sngl \<langle>lv, l, a, r\<rangle>" "lv = lvl (adjust \<langle>lv, l, a, r\<rangle>)"
+  shows "sngl (adjust \<langle>lv, l, a, r\<rangle>)" 
+using assms proof (cases rule: pre_cases)
+  case rDown
+  thus ?thesis using assms(2,3) unfolding adjust_def
+    by (auto simp add: skew_case) (auto split: tree.split)
+qed (auto simp: adjust_def skew_case split_case split: tree.split)
+
+definition "post_del t t' ==
+  invar t' \<and>
+  (lvl t' = lvl t \<or> lvl t' + 1 = lvl t) \<and>
+  (lvl t' = lvl t \<and> sngl t \<longrightarrow> sngl t')"
+
+lemma pre_adj_if_postR:
+  "invar\<langle>lv, l, a, r\<rangle> \<Longrightarrow> post_del r r' \<Longrightarrow> pre_adjust \<langle>lv, l, a, r'\<rangle>"
+by(cases "sngl r")
+  (auto simp: pre_adjust.simps post_del_def invar.simps(2) elim: sngl.elims)
+
+lemma pre_adj_if_postL:
+  "invar\<langle>lv, l, a, r\<rangle> \<Longrightarrow> post_del l l' \<Longrightarrow> pre_adjust \<langle>lv, l', b, r\<rangle>"
+by(cases "sngl r")
+  (auto simp: pre_adjust.simps post_del_def invar.simps(2) elim: sngl.elims)
+
+lemma post_del_adjL:
+  "\<lbrakk> invar\<langle>lv, l, a, r\<rangle>; pre_adjust \<langle>lv, l', b, r\<rangle> \<rbrakk>
+  \<Longrightarrow> post_del \<langle>lv, l, a, r\<rangle> (adjust \<langle>lv, l', b, r\<rangle>)"
+unfolding post_del_def
+by (metis invar_adjust lvl_adjust sngl_NodeI sngl_adjust lvl.simps(2))
+
+lemma post_del_adjR:
+assumes "invar\<langle>lv, l, a, r\<rangle>" "pre_adjust \<langle>lv, l, a, r'\<rangle>" "post_del r r'"
+shows "post_del \<langle>lv, l, a, r\<rangle> (adjust \<langle>lv, l, a, r'\<rangle>)"
+proof(unfold post_del_def, safe del: disjCI)
+  let ?t = "\<langle>lv, l, a, r\<rangle>"
+  let ?t' = "adjust \<langle>lv, l, a, r'\<rangle>"
+  show "invar ?t'" by(rule invar_adjust[OF assms(2)])
+  show "lvl ?t' = lvl ?t \<or> lvl ?t' + 1 = lvl ?t"
+    using lvl_adjust[OF assms(2)] by auto
+  show "sngl ?t'" if as: "lvl ?t' = lvl ?t" "sngl ?t"
+  proof -
+    have s: "sngl \<langle>lv, l, a, r'\<rangle>"
+    proof(cases r')
+      case Leaf thus ?thesis by simp
+    next
+      case Node thus ?thesis using as(2) assms(1,3)
+      by (cases r) (auto simp: post_del_def)
+    qed
+    show ?thesis using as(1) sngl_adjust[OF assms(2) s] by simp
+  qed
+qed
+
+declare prod.splits[split]
+
+theorem post_del_max:
+ "\<lbrakk> invar t; (t', x) = del_max t; t \<noteq> Leaf \<rbrakk> \<Longrightarrow> post_del t t'"
+proof (induction t arbitrary: t' rule: del_max.induct)
+  case (2 lv l a lvr rl ra rr)
+  let ?r =  "\<langle>lvr, rl, ra, rr\<rangle>"
+  let ?t = "\<langle>lv, l, a, ?r\<rangle>"
+  from "2.prems"(2) obtain r' where r': "(r', x) = del_max ?r"
+    and [simp]: "t' = adjust \<langle>lv, l, a, r'\<rangle>" by auto
+  from  "2.IH"[OF _ r'] \<open>invar ?t\<close> have post: "post_del ?r r'" by simp
+  note preR = pre_adj_if_postR[OF \<open>invar ?t\<close> post]
+  show ?case by (simp add: post_del_adjR[OF "2.prems"(1) preR post])
+qed (auto simp: post_del_def)
+
+theorem post_delete: "invar t \<Longrightarrow> post_del t (delete x t)"
+proof (induction t)
+  case (Node lv l a r)
+
+  let ?l' = "delete x l" and ?r' = "delete x r"
+  let ?t = "Node lv l a r" let ?t' = "delete x ?t"
+
+  from Node.prems have inv_l: "invar l" and inv_r: "invar r" by (auto)
+
+  note post_l' = Node.IH(1)[OF inv_l]
+  note preL = pre_adj_if_postL[OF Node.prems post_l']
+
+  note post_r' = Node.IH(2)[OF inv_r]
+  note preR = pre_adj_if_postR[OF Node.prems post_r']
+
+  show ?case
+  proof (cases rule: linorder_cases[of x a])
+    case less
+    thus ?thesis using Node.prems by (simp add: post_del_adjL preL)
+  next
+    case greater
+    thus ?thesis using Node.prems by (simp add: post_del_adjR preR post_r')
+  next
+    case equal
+    show ?thesis
+    proof cases
+      assume "l = Leaf" thus ?thesis using equal Node.prems
+        by(auto simp: post_del_def invar.simps(2))
+    next
+      assume "l \<noteq> Leaf" thus ?thesis using equal
+        by simp (metis Node.prems inv_l post_del_adjL post_del_max pre_adj_if_postL)
+    qed
+  qed
+qed (simp add: post_del_def)
+
+declare invar_2Nodes[simp del]
+
 
 subsection "Functional Correctness"
+
 
 subsubsection "Proofs for insert"
 
@@ -103,28 +464,28 @@ lemma inorder_insert:
   "sorted(inorder t) \<Longrightarrow> inorder(insert x t) = ins_list x (inorder t)"
 by(induction t) (auto simp: ins_list_simps inorder_split inorder_skew)
 
+
 subsubsection "Proofs for delete"
 
-lemma del_maxD:
-  "\<lbrakk> del_max t = (t',x); t \<noteq> Leaf \<rbrakk> \<Longrightarrow> inorder t' @ [x] = inorder t"
-by(induction t arbitrary: t' rule: del_max.induct)
-  (auto simp: sorted_lems split: prod.splits)
-
-lemma inorder_adjust: "t \<noteq> Leaf \<Longrightarrow> inorder(adjust t) = inorder t"
+lemma inorder_adjust: "t \<noteq> Leaf \<Longrightarrow> pre_adjust t \<Longrightarrow> inorder(adjust t) = inorder t"
 by(induction t)
-  (auto simp: adjust_def inorder_skew inorder_split split: tree.splits)
+  (auto simp: adjust_def inorder_skew inorder_split invar.simps(2) pre_adjust.simps
+     split: tree.splits)
+
+lemma del_maxD:
+  "\<lbrakk> del_max t = (t',x); t \<noteq> Leaf; invar t \<rbrakk> \<Longrightarrow> inorder t' @ [x] = inorder t"
+by(induction t arbitrary: t' rule: del_max.induct)
+  (auto simp: sorted_lems inorder_adjust pre_adj_if_postR post_del_max split: prod.splits)
 
 lemma inorder_delete:
-  "sorted(inorder t) \<Longrightarrow> inorder(delete x t) = del_list x (inorder t)"
+  "invar t \<Longrightarrow> sorted(inorder t) \<Longrightarrow> inorder(delete x t) = del_list x (inorder t)"
 by(induction t)
-  (auto simp: del_list_simps inorder_adjust del_maxD split: prod.splits)
+  (auto simp: del_list_simps inorder_adjust pre_adj_if_postL pre_adj_if_postR 
+              post_del_max post_delete del_maxD split: prod.splits)
 
-
-subsection "Overall correctness"
-
-interpretation Set_by_Ordered
+interpretation I: Set_by_Ordered
 where empty = Leaf and isin = isin and insert = insert and delete = delete
-and inorder = inorder and inv = "\<lambda>_. True"
+and inorder = inorder and inv = invar
 proof (standard, goal_cases)
   case 1 show ?case by simp
 next
@@ -133,6 +494,12 @@ next
   case 3 thus ?case by(simp add: inorder_insert)
 next
   case 4 thus ?case by(simp add: inorder_delete)
-qed auto
+next
+  case 5 thus ?case by(simp)
+next
+  case 6 thus ?case by(simp add: invar_insert)
+next
+  case 7 thus ?case using post_delete by(auto simp: post_del_def)
+qed
 
 end
