src/HOL/Data_Structures/AA_Map.thy
@@ -1,6 +1,6 @@
 (* Author: Tobias Nipkow *)
 
-section "AA Implementation of Maps"
+section "AA Tree Implementation of Maps"
 
 theory AA_Map
 imports
@@ -26,21 +26,190 @@ fun delete :: "'a::cmp \<Rightarrow> ('a*'b) aa_tree \<Rightarrow> ('a*'b) aa_tr
             else let (l',ab') = del_max l in adjust (Node lv l' ab' r)))"
 
 
+subsection "Invariance"
+
+subsubsection "Proofs for insert"
+
+lemma lvl_update_aux:
+  "lvl (update x y t) = lvl t \<or> lvl (update x y t) = lvl t + 1 \<and> sngl (update x y t)"
+apply(induction t)
+apply (auto simp: lvl_skew)
+apply (metis Suc_eq_plus1 lvl.simps(2) lvl_split lvl_skew)+
+done
+
+lemma lvl_update: obtains
+  (Same) "lvl (update x y t) = lvl t" |
+  (Incr) "lvl (update x y t) = lvl t + 1" "sngl (update x y t)"
+using lvl_update_aux by fastforce
+
+declare invar.simps(2)[simp]
+
+lemma lvl_update_sngl: "invar t \<Longrightarrow> sngl t \<Longrightarrow> lvl(update x y t) = lvl t"
+proof (induction t rule: update.induct)
+  case (2 x y lv t1 a b t2)
+  consider (LT) "x < a" | (GT) "x > a" | (EQ) "x = a" 
+    using less_linear by blast 
+  thus ?case proof cases
+    case LT
+    thus ?thesis using 2 by (auto simp add: skew_case split_case split: tree.splits)
+  next
+    case GT
+    thus ?thesis using 2 proof (cases t1)
+      case Node
+      thus ?thesis using 2 GT  
+        apply (auto simp add: skew_case split_case split: tree.splits)
+        by (metis less_not_refl2 lvl.simps(2) lvl_update_aux n_not_Suc_n sngl.simps(3))+ 
+    qed (auto simp add: lvl_0_iff)
+  qed simp
+qed simp
+
+lemma lvl_update_incr_iff: "(lvl(update a b t) = lvl t + 1) \<longleftrightarrow>
+  (EX l x r. update a b t = Node (lvl t + 1) l x r \<and> lvl l = lvl r)"
+apply(cases t)
+apply(auto simp add: skew_case split_case split: if_splits)
+apply(auto split: tree.splits if_splits)
+done
+
+lemma invar_update: "invar t \<Longrightarrow> invar(update a b t)"
+proof(induction t)
+  case (Node n l xy r)
+  hence il: "invar l" and ir: "invar r" by auto
+  obtain x y where [simp]: "xy = (x,y)" by fastforce
+  note N = Node
+  let ?t = "Node n l xy r"
+  have "a < x \<or> a = x \<or> x < a" by auto
+  moreover
+  { assume "a < x"
+    note iil = Node.IH(1)[OF il]
+    have ?case
+    proof (cases rule: lvl_update[of a b l])
+      case (Same) thus ?thesis
+        using \<open>a<x\<close> invar_NodeL[OF Node.prems iil Same]
+        by (simp add: skew_invar split_invar del: invar.simps)
+    next
+      case (Incr)
+      then obtain t1 w t2 where ial[simp]: "update a b l = Node n t1 w t2"
+        using Node.prems by (auto simp: lvl_Suc_iff)
+      have l12: "lvl t1 = lvl t2"
+        by (metis Incr(1) ial lvl_update_incr_iff tree.inject)
+      have "update a b ?t = split(skew(Node n (update a b l) xy r))"
+        by(simp add: \<open>a<x\<close>)
+      also have "skew(Node n (update a b l) xy r) = Node n t1 w (Node n t2 xy r)"
+        by(simp)
+      also have "invar(split \<dots>)"
+      proof (cases r)
+        case Leaf
+        hence "l = Leaf" using Node.prems by(auto simp: lvl_0_iff)
+        thus ?thesis using Leaf ial by simp
+      next
+        case [simp]: (Node m t3 y t4)
+        show ?thesis (*using N(3) iil l12 by(auto)*)
+        proof cases
+          assume "m = n" thus ?thesis using N(3) iil by(auto)
+        next
+          assume "m \<noteq> n" thus ?thesis using N(3) iil l12 by(auto)
+        qed
+      qed
+      finally show ?thesis .
+    qed
+  }
+  moreover
+  { assume "x < a"
+    note iir = Node.IH(2)[OF ir]
+    from \<open>invar ?t\<close> have "n = lvl r \<or> n = lvl r + 1" by auto
+    hence ?case
+    proof
+      assume 0: "n = lvl r"
+      have "update a b ?t = split(skew(Node n l xy (update a b r)))"
+        using \<open>a>x\<close> by(auto)
+      also have "skew(Node n l xy (update a b r)) = Node n l xy (update a b r)"
+        using Node.prems by(simp add: skew_case split: tree.split)
+      also have "invar(split \<dots>)"
+      proof -
+        from lvl_update_sngl[OF ir sngl_if_invar[OF \<open>invar ?t\<close> 0], of a b]
+        obtain t1 p t2 where iar: "update a b r = Node n t1 p t2"
+          using Node.prems 0 by (auto simp: lvl_Suc_iff)
+        from Node.prems iar 0 iir
+        show ?thesis by (auto simp: split_case split: tree.splits)
+      qed
+      finally show ?thesis .
+    next
+      assume 1: "n = lvl r + 1"
+      hence "sngl ?t" by(cases r) auto
+      show ?thesis
+      proof (cases rule: lvl_update[of a b r])
+        case (Same)
+        show ?thesis using \<open>x<a\<close> il ir invar_NodeR[OF Node.prems 1 iir Same]
+          by (auto simp add: skew_invar split_invar)
+      next
+        case (Incr)
+        thus ?thesis using invar_NodeR2[OF `invar ?t` Incr(2) 1 iir] 1 \<open>x < a\<close>
+          by (auto simp add: skew_invar split_invar split: if_splits)
+      qed
+    qed
+  }
+  moreover { assume "a = x" hence ?case using Node.prems by auto }
+  ultimately show ?case by blast
+qed simp
+
+subsubsection "Proofs for delete"
+
+declare invar.simps(2)[simp del]
+
+theorem post_delete: "invar t \<Longrightarrow> post_del t (delete x t)"
+proof (induction t)
+  case (Node lv l ab r)
+
+  obtain a b where [simp]: "ab = (a,b)" by fastforce
+
+  let ?l' = "delete x l" and ?r' = "delete x r"
+  let ?t = "Node lv l ab r" let ?t' = "delete x ?t"
+
+  from Node.prems have inv_l: "invar l" and inv_r: "invar r" by (auto)
+
+  note post_l' = Node.IH(1)[OF inv_l]
+  note preL = pre_adj_if_postL[OF Node.prems post_l']
+
+  note post_r' = Node.IH(2)[OF inv_r]
+  note preR = pre_adj_if_postR[OF Node.prems post_r']
+
+  show ?case
+  proof (cases rule: linorder_cases[of x a])
+    case less
+    thus ?thesis using Node.prems by (simp add: post_del_adjL preL)
+  next
+    case greater
+    thus ?thesis using Node.prems preR by (simp add: post_del_adjR post_r')
+  next
+    case equal
+    show ?thesis
+    proof cases
+      assume "l = Leaf" thus ?thesis using equal Node.prems
+        by(auto simp: post_del_def invar.simps(2))
+    next
+      assume "l \<noteq> Leaf" thus ?thesis using equal Node.prems
+        by simp (metis inv_l post_del_adjL post_del_max pre_adj_if_postL)
+    qed
+  qed
+qed (simp add: post_del_def)
+
+
 subsection {* Functional Correctness Proofs *}
 
 theorem inorder_update:
   "sorted1(inorder t) \<Longrightarrow> inorder(update x y t) = upd_list x y (inorder t)"
 by (induct t) (auto simp: upd_list_simps inorder_split inorder_skew)
 
-
 theorem inorder_delete:
-  "sorted1(inorder t) \<Longrightarrow> inorder (delete x t) = del_list x (inorder t)"
+  "\<lbrakk>invar t; sorted1(inorder t)\<rbrakk> \<Longrightarrow>
+  inorder (delete x t) = del_list x (inorder t)"
 by(induction t)
-  (auto simp: del_list_simps inorder_adjust del_maxD split: prod.splits)
+  (auto simp: del_list_simps inorder_adjust pre_adj_if_postL pre_adj_if_postR 
+              post_del_max post_delete del_maxD split: prod.splits)
 
-interpretation Map_by_Ordered
+interpretation I: Map_by_Ordered
 where empty = Leaf and lookup = lookup and update = update and delete = delete
-and inorder = inorder and inv = "\<lambda>_. True"
+and inorder = inorder and inv = invar
 proof (standard, goal_cases)
   case 1 show ?case by simp
 next
@@ -49,6 +218,12 @@ next
   case 3 thus ?case by(simp add: inorder_update)
 next
   case 4 thus ?case by(simp add: inorder_delete)
-qed auto
+next
+  case 5 thus ?case by(simp)
+next
+  case 6 thus ?case by(simp add: invar_update)
+next
+  case 7 thus ?case using post_delete by(auto simp: post_del_def)
+qed
 
 end
